$$p=\rho RT$$
$$e=c_{v}T$$
$$\frac{p_{2}}{p_{1}}=\left(\frac{T_{2}}{T_{1}}\right)^{\frac{\gamma}{\gamma-1}}=\left(\frac{\rho_{2}}{\rho_{1}}\right)^{\gamma}$$
$$\begin{align*}
const.&= \frac{p_{1}}{\rho_{1}}+ \frac{1}{2}V_{1}^{2}+C_{v}T_{1}\\
&= \frac{p_{2}}{\rho_{1}}+ \frac{1}{2}V_{2}^{2}+C_{v}T_{2}
\end{align*}$$
$$\begin{align*}
const.&= \frac{p_{1}}{\rho_{1}}+ \frac{1}{2}V_{1}^{2}+C_{v}T_{1}\\
&= \frac{p_{2}}{\rho_{1}}+ \frac{1}{2}V_{2}^{2}+C_{v}T_{2}
\end{align*}$$
$$h_{0}=h+ \frac{1}{2}V^{2}=const.$$
$$T_{0}=T\left(1+\frac{(\gamma-1)M^{2}}{2}\right)$$
$$\frac{p_{02}}{p_{01}}=e^{-(\frac{s_{2}-s_{1}}{R})}$$
$$a^{2}=\frac{\gamma p}{\rho}\Rightarrow \boxed{a=\sqrt{\gamma RT}}$$$$
C_{p}= \frac{p-p_{\infty}}{q_{\infty}}=\frac{2(p/p_{\infty}-1)}{\gamma M_{\infty}^{2}}$$
